proofs/core/RecFun.v
@@ -236,22 +236,451 @@ Require Import Hlist.
 (*TODO: where do we need the bodies?*)
 Variable (fs: list fn) (ps: list pn).
 Print well_founded.
+
+(*Let's try this at first*)
+Inductive list_rel {A: Type} : list A -> list A -> Prop :=
+  | LR_constr: forall x t l,
+    l = x :: t ->
+    list_rel t l.
+
+Lemma list_rel_wf: forall A, well_founded (@list_rel A).
+Proof.
+  intros. unfold well_founded. intros. induction a; simpl.
+  constructor. intros. inversion H; subst. inversion H0.
+  constructor. intros. inversion H; subst.
+  inversion H0; subst. apply IHa.
+Defined.
+
+(*OK, how about mutual recursive type*)
+Unset Elimination Schemes.
+Inductive rosetree {A: Type} : Type :=
+  | Leaf: A -> rosetree
+  | Node: roselist -> rosetree
+with roselist {A: Type} : Type :=
+  | RL_nil : roselist
+  | RL_cons: rosetree -> roselist -> roselist.
+Set Elimination Schemes.
+
+Scheme rosetree_ind := Induction for rosetree Sort Prop with
+roselist_ind := Induction for roselist Sort Prop.
+
+
+Inductive Either (A B: Type) : Type :=
+  | Left: A -> Either A B
+  | Right: B -> Either A B.
+
+
+(*Now can we get a wf relation?*)
+Inductive rose_rel {A: Type} : Either (@rosetree A) (@roselist A) -> 
+  Either (@rosetree A) (@roselist A) -> Prop :=
+  | RR_constr1: forall rt rl,
+    rt = Node rl ->
+    rose_rel (Right _ _ rl) (Left _ _ rt)
+  | RR_constr2: forall rt rl x,
+    rl = RL_cons rt x ->
+    rose_rel (Left _ _ rt) (Right _ _ rl)
+  | RR_constr3: forall rl1 rl2 x,
+    rl1 = RL_cons x rl2 ->
+    rose_rel (Right _ _ rl2) (Right _ _ rl1).
+
+Set Bullet Behavior "Strict Subproofs".
+
+Definition prop_either {A B: Type} (P: A -> Prop) (P1: B -> Prop):
+  Either A B -> Prop :=
+  fun x =>
+  match x with
+  | Left y => P y
+  | Right y => P1 y
+  end.
+
+(*Lemma rose_tree_list_ind {A: Type} (P: @rosetree A -> Prop)
+(P0: roselist -> Prop)
+(Hleaf: forall a, P (Leaf a))
+(Hnode: forall r, P0 r -> P(Node r))
+(Hnil: P0 RL_nil)
+(Hcons: forall r, P r -> forall r0, P0 r0 -> P0 (RL_cons r r0)):
+*)
+
+Definition either_rose_ind {A: Type} (P: @rosetree A -> Prop)
+  (P0: roselist -> Prop) (P3: Either rosetree roselist -> Prop)
+  (Hleaf: forall a, P (Leaf a))
+  (Hnode: forall r, P0 r -> P(Node r))
+  (Hnil: P0 RL_nil)
+  (Hcons: forall r, P r -> forall r0, P0 r0 -> P0 (RL_cons r r0))
+  (Hp3_1: forall x, P3 (Left _ _ x) <-> P x)
+  (Hp3_2: forall x, P3 (Right _ _ x) <-> P0 x)
+  :
+  forall (x: Either rosetree roselist), P3 x.
+Proof.
+  intros. destruct x.
+  - rewrite Hp3_1. apply rosetree_ind with(P0:=P0); auto.
+  - rewrite Hp3_2. apply roselist_ind with(P:=P); auto.
+Qed.
+
+Lemma rose_rel_wf: forall A, well_founded (@rose_rel A).
+Proof.
+  intros. unfold well_founded.
+  apply either_rose_ind with(P:= fun x => Acc rose_rel (Left _ _ x))
+    (P0:= fun y => Acc rose_rel (Right _ _ y)); intros.
+  - constructor. intros. inversion H; subst. inversion H2.
+  - constructor. intros. inversion H0; subst.
+    inversion H3; subst. apply H.
+  - constructor. intros. inversion H; subst; inversion H2.
+  - constructor. intros. inversion H1; subst;
+    inversion H4; subst; assumption.
+  - reflexivity.
+  - reflexivity.
+Qed.
+
+Instance rose_rel_wf': WellFounded
+(Telescopes.tele_measure (Telescopes.tip (Either rosetree roselist))
+   (Either rosetree (@roselist nat)) (fun o : Either rosetree roselist => o)
+   rose_rel).
+Proof.
+  unfold WellFounded. apply rose_rel_wf.
+Defined. 
+
+Equations rose_size (*{A: Type}*) (o: Either (@rosetree nat) (@roselist nat)) : nat
+  by wf o (@rose_rel nat) :=
+  rose_size (Left (Leaf x)) := 1;
+  rose_size (Left (Node l)) := rose_size (Right _ _ l);
+  rose_size (Right RL_nil) := 0;
+  rose_size (Right (RL_cons t ls)) :=
+    rose_size (Left _ _ t) + rose_size (Right _ _ ls).
+Next Obligation.
+  constructor. reflexivity.
+Defined.
+Next Obligation.
+  eapply RR_constr2. reflexivity.
+Defined.
+Next Obligation.
+  eapply RR_constr3. reflexivity.
+Defined.
+
+(*Next, want to make polymoprhic by including type there*)
+(*Now can we get a wf relation?*)
+Inductive rose_rel2: {A: Type & Either (@rosetree A) (@roselist A)} -> 
+  {A: Type & Either (@rosetree A) (@roselist A)} -> Prop :=
+  | RR_constr1': forall A rt rl,
+    rt = Node rl ->
+    rose_rel2 (existT _ A (Right _ _ rl)) (existT _ A (Left _ _ rt))
+  | RR_constr2': forall A rt rl x,
+    rl = RL_cons rt x ->
+    rose_rel2 (existT _ A (Left _ _ rt)) (existT _ A (Right _ _ rl))
+  | RR_constr3': forall A rl1 rl2 x,
+    rl1 = RL_cons x rl2 ->
+    rose_rel2 (existT _ A (Right _ _ rl2)) (existT _ A (Right _ _ rl1)).
+
+Lemma rose_rel2_wf:well_founded (rose_rel2).
+Proof.
+  unfold well_founded.
+  (*Can intros A because it is fixed (by definition) - will
+    this be true in why3 types?*)
+  intros [A o]. revert o.
+  apply either_rose_ind with(P:= fun x => Acc rose_rel2 (existT _ A (Left _ _ x)))
+    (P0:= fun y => Acc rose_rel2 (existT _ A (Right _ _ y))); intros.
+  - constructor. intros. inversion H; subst. inversion H3.
+  - constructor. intros. inversion H0; subst.
+    inversion H4; subst.
+    (*In real one, will be able to have decidable types
+    (quantify with vty)*)
+    apply Eqdep.EqdepTheory.inj_pair2 in H2.
+    (*Hmm, annoying things with existT - ToDO*)
+    (*apply Eqdep_dec.inj_pair2_eq_dec in H2.*)
+    subst. assumption.
+  - constructor. intros. inversion H; subst; inversion H3.
+  - constructor. intros. inversion H1; subst; inversion H5;
+    apply Eqdep.EqdepTheory.inj_pair2 in H3;
+    apply Eqdep.EqdepTheory.inj_pair2 in H4; subst; assumption.
+  - reflexivity.
+  - reflexivity.
+Qed.
+
+Instance rose_rel2_wf': WellFounded
+(Telescopes.tele_measure
+   (Telescopes.tip {A : Type & Either rosetree roselist})
+   {A : Type & Either rosetree roselist}
+   (fun o : {A : Type & Either rosetree roselist} => o) rose_rel2).
+Proof.
+  apply rose_rel2_wf.
+Defined.
+
+Equations rose_size2 (*{A: Type}*) 
+  (o: {A: Type & Either (@rosetree A) (@roselist A) }) : nat
+  by wf o (rose_rel2) :=
+  rose_size2 (existT _ A (Left (Leaf x))) := 1;
+  rose_size2 (existT _ A (Left (Node l))) := 
+    rose_size2 (existT _ A (Right _ _ l));
+  rose_size2 (existT _ A (Right RL_nil)) := 0;
+  rose_size2 (existT _ A (Right (RL_cons t ls))) :=
+    rose_size2 (existT _ A (Left _ _ t)) + rose_size2 (existT _ A (Right _ _ ls)).
+Next Obligation.
+  constructor. reflexivity.
+Defined.
+Next Obligation.
+  eapply RR_constr2'. reflexivity.
+Defined.
+Next Obligation.
+  eapply RR_constr3'. reflexivity.
+Defined.
+
+(*OK, so now I want to try a non-terminating function
+  using my approach, and see where it goes wrong*)
+
+(*Idea: function on two lists, pattern match on both*)
+(*
+Fixpoint foo {A: Type} (l1 l2: list A)  : list A :=
+  match l1, l2 with
+  | x1 :: t1, x2 :: t2 => foo t1 (x1 :: x2 :: t2)
+  | _, x2 :: t2 => foo [x2] t2
+  | _, _ => nil
+  
+  end.
+*)
+
+(*Now we will define a well-founded relation on
+  pairs of lists*)
+(*Is this well-founded?*)
+Definition pairlist_rel : 
+  (bool * (list nat * list nat)) -> (bool * (list nat * list nat)) -> Prop :=
+  fun x1 x2 =>
+    match x1, x2 with
+    | (b1, (l11, l12)), (b2, (l21, l22)) =>
+    list_rel (if b1 then l11 else l12) (if b2 then l21 else l22)
+    end.
+
+(*
+Lemma pairlist_rel_wf: well_founded pairlist_rel.
+
+Good, we can't prove this - but what should we do?
+  Key idea: every invocation of the SAME function must use the same
+  index.
+
+  For non mutual - we have a single index, look at
+  arg_lists, compare this single (fixed) index.
+  This should be prvable: example 
+*)
+Definition pairlist_fstrel: (bool * (list nat * list nat)) ->
+  (bool * (list nat * list nat)) -> Prop :=
+  fun x1 x2 =>
+  match x1, x2 with
+    | (b1, (l11, l12)), (b2, (l21, l22)) =>
+    if b1 && b2 then list_rel l11 l21 else False
+  end.
+
+Lemma pairlist_rel_wf: well_founded pairlist_fstrel.
+Proof.
+  unfold well_founded. intros.
+  destruct a as [b [l1 l2]].
+  revert l2.
+  (*Key: Only need to generalize/do induction on l1*)
+  induction l1; simpl.
+  - constructor. intros. unfold pairlist_fstrel in H.
+    destruct y; destruct p. destruct b0; destruct b; inversion H.
+    inversion H0.
+  - constructor. intros. unfold pairlist_fstrel in H.
+    destruct y; destruct p. destruct b0; destruct b; inversion H.
+    subst. inversion H0; subst.
+    apply IHl1.
+Qed.
+
+(*For the mutual case, we will need a different index
+  for each function*)
+(*How can we prove that this is WF? I guess our relation is
+  something like:
+  {f: funsym & funsym_sigma_args sigma f}
+  or so, then internally we use the index
+  How can we model this here?
+  *) 
+
+(*I think - do single first, then worry about mutual when we
+  see what we need - should be OK*)
+
+(*TODO: first, we will do this for the non-mutual case with
+  just a single function. Then, we will add mutual recursion*)
+
+(*Let's define the relation*)
+Search mk_adts.
+Print pi_dom.
+Require Import Denotational.
+Check is_sort_adt_spec.
+Print match_val_single.
+Check funargs_to_vals.
+Check is_sort_adt_spec.
+Print typesym_to_sort.
+Check typesym_to_sort_proof.
+Search m_params s_params.
+Print val.
+Locate adts.
+Print Semantics.adts.
+
+Inductive adt_smaller: {t: {ty: vty | valid_type sigma ty} & 
+  domain (val (proj1_sig t))} ->
+  {t: {ty: vty | valid_type sigma ty} & domain (val (proj1_sig t))} -> Prop :=
+  | ADT_small: forall x1 x2 vv ty t1 t2 Hval1 Hval2 d1 d2 m a ts srts
+    (*NOTE: in general, not all same type, need 2 tys*)
+    (Hx1: x1 = existT _ (exist (valid_type sigma) ty Hval2) d1)
+    (Hx2: x2 = existT _ (exist _ ty Hval1) d2)
+    (Hisadt: is_sort_adt (val ty) = 
+      Some (m, a, ts, srts)),
+    let adt_spec := (is_sort_adt_spec _ _ _ _ _ _ Hisadt) in
+    let Hseq := proj1 adt_spec in
+    let a_in := proj1 (proj2 adt_spec) in
+    let m_in :=  proj1 (proj2 (proj2 adt_spec)) in
+    (*cast to adt type*)
+    let adt : adt_rep m srts (dom_aux pd) a a_in :=
+      scast (Semantics.adts pd m srts a a_in) (dom_cast _ Hseq d2) in 
+    (*need lengths lemma*)
+    let lengths_eq : length srts = length (m_params m) :=
+      adt_srts_length_eq gamma_valid Hisadt Hval2 in 
+    (*Now we get the constructor c and arg_list a such
+      that d2 = [[c(a)]]*)
+    let Hrep := find_constr_rep gamma_valid m m_in srts lengths_eq
+      (dom_aux pd) a a_in (Semantics.adts pd m srts) 
+        (all_unif m m_in) adt in
+    let c : funsym := projT1 Hrep in
+    let c_in : constr_in_adt c a :=
+      fst (proj1_sig (projT2 Hrep)) in
+    let args : arg_list domain (funsym_sigma_args c srts) := 
+      snd (proj1_sig (projT2 Hrep)) in
+    (*Then it must be the case that d1 equals
+      one of the arguments in args*)
+      (*TODO: need lengths of (s_params c)*)
+    let lens : length (s_params c) = length (m_params m) :=
+      f_equal (@length _) (adt_constr_params gamma_valid m_in a_in c_in) in
+    let lens': length (s_params c) = length srts :=
+      eq_trans lens (eq_sym lengths_eq) in
+    (*TODO: convert args list bc they are sorts - is there better
+      way than all this? Maybe not - this is similar to match*)
+    let val_args := funargs_to_vals pd vt c (map sort_to_ty srts) _ 
+      (*lens'*) args in
+    exists i, i < hlength val_args /\
+    d2 = hnth i val_args.
+
+
+    (*TODO: make more generic function to convert between
+    funsym_sigma_args and val list*)
+    
+
+
+
+      match (is_sort_adt_spec _ _ _ _ _ Hisadt) with
+      | conj Hseq (conj a_in (conj m_in Htseq)) =>
+        (*We cast to get an ADT, now that we know that this actually is
+          an ADT*)
+        let adt : adt_rep m srts (dom_aux pd) a a_in :=
+          scast (adts pd m srts a a_in) (dom_cast _ Hseq d) in
+       
+        (*Need a lemma about lengths for [find_constr_rep]*)
+        let lengths_eq : length srts = length (m_params m) := 
+          adt_srts_length_eq Hisadt Hval in
+
+        (*The key part: get the constructor c and arg_list a
+          such that d = [[c(a)]]*)
+        let Hrep := find_constr_rep gamma_valid m m_in srts lengths_eq 
+          (dom_aux pd) a a_in (adts pd m srts) 
+          (all_unif m m_in) adt in
+
+
+    () 
+
+
+
+adts : forall (m : mut_adt) (srts : list sort) 
+             (a : alg_datatype) (Hin : adt_in_mut a m),
+           IndTypes.domain dom_aux (typesym_to_sort (adt_name a) srts) =
+           adt_rep m srts dom_aux a Hin
+
 (*Assume we have some relation (TODO: need to find out which)*)
 (*TODO: on domains, will have precondition that they are adt*)
-Axiom adt_smaller: forall (ty: vty),
-(domain (val ty)) ->
-(domain (val ty)) ->
-Prop.
-Axiom adt_smaller_wf: forall (ty: vty),
-  well_founded (adt_smaller ty).
+Axiom adt_smaller:
+  (*We hide the type because they may not be the same,
+    for instance with a mutually recursive type*)
+  {t: vty & domain (val t)} ->
+  {t: vty & domain (val t)} -> Prop.
+Axiom adt_smaller_wf: well_founded adt_smaller.
+Require Import Denotational.
+Check funsym_subst_eq.
+Check v_subst.
+
+(*TODO: think we will need something better than
+  [get_arg_list] - we will want direct, invertible
+  conversion functions*)
+
+(*Because input to this will be with funsym_sigma_args
+  but our inductive relation should really use
+  an arg_list of (domain (val x))*)
+(*Want generic way to convert between them*)
+
+(*Next, we lift this to (nat, [arg_list]) pairs,
+  where the nat represents the index of the smaller
+  argument*)
+(*TODO: do we need proof nat is in bounds?*)
+Definition arg_list_smaller:
+  {x: { t: nat * list sort | fst t < length (snd t) } & 
+    arg_list domain (snd (proj1_sig x))} ->
+  {x: { t: nat * list sort | fst t < length (snd t) } & 
+  arg_list domain (snd (proj1_sig x))} -> 
+  Prop.
+Proof.
+  intros x1 x2.
+  destruct x1 as [[[n1 s1] Hn1] al1].
+  destruct x2 as [[[n2 s2] Hn2] al2].
+  Check hnth.
+  remember (hnth n1 al1 s_int (dom_int pd)) as y.
+  simpl in y.
+  remember (hnth n2 al2 s_int (dom_int pd)) as z.
+  simpl in z.
+  Print existT.
+  (*Ah, we need a list we are using val for*)
+  (*See how Denotational does it*)
+  apply (adt_smaller (existT _ (nth n1 s1 s_int)  y) (existT _ z)).
+  Print domain.
+  Print dom_aux.
+  Search dom_aux s_int.
+  simpl in y.
+  (nat * {s: list sort & arg_list domain s}) ->
+  (nat * {s: list sort & arg_list domain s}) ->
+  Prop.
+intros x1 x2.
+
 
 (*Need to lift this to arg list*)
 (*TODO: relate to above, need def*)
-Axiom arg_list_smaller: forall (idx: nat) (srts: list sort),
+(*TODO: do we need index here? Or can we use exists?*)
+Axiom arg_list_smaller: forall (srts: list sort),
   arg_list domain srts ->
   arg_list domain srts -> Prop.
-Axiom arg_list_smaller_wf : forall (idx: nat) (srts: list sort),
-  well_founded (arg_list_smaller idx srts).
+Axiom arg_list_smaller_wf : forall (srts: list sort),
+  well_founded (arg_list_smaller srts).
+
+  (*Hmm, think about this*)
+  (*What I think: we need an index, we need to say
+    that the specific type argument is smaller
+    (arg lists may not be same type)
+    But even these may not be same type
+    so our relation might need to be on 2 things of different
+    types or like {x : ty & domain (val ty)}
+    i think (bc of non-uniformity) tihs is caused by
+    mutually-recursive types
+    *)
+
+  (*try to do on paper, let's see*)
+Definition input_smaller: forall i1 i2 srts1 srts2,
+  {b : bool &
+         {t
+         : {i : nat | i < (if b then i1 else i2)} &
+         arg_list domain
+           (if b then srts1 else srts2)}} ->
+  {b : bool &
+         {t
+         : {i : nat | i < (if b then i1 else i2)} &
+         arg_list domain
+           (if b then srts1 else srts2)}} ->
+  Prop := fun i1 i2 srts1 srts2 x1 x2 =>
+  arg_list_smaller _ (projT2 (projT2 x1)) (projT2 (projT2 x2)). 
+Proof.
+
 
 (*TODO: need to prove our relation on pairs is well-founded*)
 
@@ -286,6 +715,7 @@ Definition ps_d : predsym :=
 Definition fs_d : funsym :=
     Build_funsym EmptyString nil nil vty_int eq_refl eq_refl eq_refl.
 
+(*This is the version for the function body*)
 Definition build_indfun (small: list vsymbol) 
 (hd: string) (hd_ty: vty)
 (hd_idx: nat) (vv: val_vars pd vt) (body: term) (ty: vty) 
@@ -299,7 +729,7 @@ Definition build_indfun (small: list vsymbol)
 (args: {b: bool & {t: {i : nat | i < if b then length fs else length ps} &
   arg_list domain (if b then (funsym_sigma_args (nth (proj1_sig t) (map fn_name fs) fs_d) srts) 
     else (predsym_sigma_args (nth (proj1_sig t) (map pn_name ps) ps_d) srts))}}) :
-(if (projT1 args) then domain (funsym_sigma_ret (nth (proj1_sig (projT1 (projT2 args))) (map fn_name fs) fs_d) srts)
+(if (projT1 args) then domain (val ty)
   else bool).
 Proof.
   revert args.
